Examples: progress in proving standard model for PA

theories/Examples.v
@@ -1,5 +1,5 @@
 From Coq Require Import Vector.
-Require Import Base Syntax Semantics InductiveDefinitions.
+Require Import Base Syntax Semantics InductiveDefinitions LKID.
 Import VectorNotations.
 
 Inductive Func__PA :=
@@ -101,8 +101,57 @@ Inductive Φ__PA : @production Σ__PA -> Prop :=
 | ID_E_succ : Φ__PA PA_prod_E_succ
 | ID_O_succ : Φ__PA PA_prod_O_succ.
 
-Inductive IsNat : nat -> Prop :=
-| isNat : forall n, IsNat n.
+Inductive NAT : nat -> Prop :=
+| NO : NAT 0
+| NS : forall n, NAT n -> NAT (S n).
+
+Lemma NAT_all : forall n, NAT n.
+  induction n; constructor; auto.
+Qed.
+
+Inductive EVEN : nat -> Prop :=
+| EO : EVEN 0
+| ES : forall n, ODD n -> EVEN (S n)
+with ODD : nat -> Prop :=
+| OS : forall n, EVEN n -> ODD (S n).
+
+Section Eind.
+  Context (P : nat -> Prop).
+  Context (HO : P O).
+  Context (HS : forall n, EVEN n -> P n -> P (S (S n))).
+  Definition EVEN_ind2 : forall n, EVEN n -> P n.
+    fix IND 1. intros n HE. destruct n.
+    - apply HO.
+    - destruct n.
+      + inversion HE; inversion H0.
+      + apply HS.
+        * inversion HE. inversion H0. assumption.
+        * apply IND. inversion HE. inversion H0. assumption.
+  Defined.
+End Eind.
+
+Section Oind.
+  Context (P : nat -> Prop).
+  Context (HO : P 1).
+  Context (HS : forall n, ODD n -> P n -> P (S (S n))).
+  Definition ODD_ind2 : forall n, ODD n -> P n.
+    fix IND 1. intros n HODD. destruct n.
+    - inversion HODD.
+    - destruct n.
+      + apply HO.
+      + apply HS.
+        * inversion HODD. inversion H0. assumption.
+        * apply IND. inversion HODD. inversion H0. assumption.
+  Defined.
+End Oind.
+
+Lemma pair_induction (P : nat -> Prop) :
+  P 0 -> P 1 -> (forall n, P n -> P (S n) -> P (S (S n))) -> forall n, P n.
+Proof.
+  intros H0 H1 HS n.
+  enough (P n /\ P (S n)) by tauto.
+  induction n; intuition.
+Qed.
 
 Definition M__PA : @structure Σ__PA.
   refine (Build_structure nat _ _ _).
@@ -114,10 +163,99 @@ Definition M__PA : @structure Σ__PA.
   - intros []. cbn. intros args.
     exact (V.hd args = V.hd (V.tl args)).
   - intros []; cbn; intros args.
-    + exact (IsNat (V.hd args)).
-    + exact (Nat.Even (V.hd args)).
-    + exact (Nat.Odd (V.hd args)).
+    + exact (NAT (V.hd args)).
+    + exact (EVEN (V.hd args)).
+    + exact (ODD (V.hd args)).
 Defined.
 
+Import VectorNotations.
+
+Lemma NAT_φ_Φ_ω: forall n, @φ_Φ_ω Σ__PA M__PA Φ__PA PA_N (V.cons n V.nil).
+  induction n.
+  - exists 1. unfold φ_Φ_n, φ_Φ, φ_P. exists PA_prod_N_zero, (conj eq_refl ID_N_zero).
+    unfold φ_pr. cbn. eexists; intuition.
+  - destruct IHn as [α IH]. exists (S α).
+    cbn. unfold φ_Φ, φ_P. exists PA_prod_N_succ, (conj eq_refl ID_N_succ).
+    unfold φ_pr. cbn. intuition. exists (fun x => match x with
+                                          | 0 => n
+                                          | S y => x
+                                          end).
+    intuition. destruct P; cbn.
+    + apply inj_pair2 in H0. subst. cbn. assumption.
+    + inversion H0.
+    + inversion H0.
+      Unshelve. intros n. exact n.
+Qed.
+
+Lemma EVEN_φ_Φ_ω : forall n, EVEN n -> @φ_Φ_ω Σ__PA M__PA Φ__PA PA_E (V.cons n V.nil).
+Proof.
+  intros n HE. induction HE using EVEN_ind2.
+  - exists 1. unfold φ_Φ_n, φ_Φ, φ_P. exists PA_prod_E_zero, (conj eq_refl ID_E_zero).
+    unfold φ_pr. cbn. eexists; intuition.
+  - destruct IHHE as [a Ha]. exists (S (S a)); cbn.
+    unfold φ_Φ at 1. unfold φ_P at 1.
+    exists PA_prod_E_succ, (conj eq_refl ID_E_succ); cbn.
+    unfold φ_pr. cbn. exists (fun x => match x with
+                               | O => S n
+                               | S y => x
+                               end); intuition.
+    destruct P; try discriminate.
+    apply inj_pair2 in H0; subst; cbn.
+    unfold φ_Φ, φ_P. exists PA_prod_O_succ, (conj eq_refl ID_O_succ); cbn.
+    unfold φ_pr; cbn. exists (fun x => match x with
+                               | O => n
+                               | S y => x
+                               end); intuition.
+    destruct P; try discriminate.
+    apply inj_pair2 in H0; subst; cbn. assumption.
+    Unshelve.
+    intros n; exact n.
+Qed.
+
+Lemma φ_Φ_ω_EVEN : forall n, @φ_Φ_ω Σ__PA M__PA Φ__PA PA_E (V.cons n V.nil) -> EVEN n.
+Proof.
+  intros n [α Hα].
+  revert Hα. induction α.
+  - inversion 1.
+  - inversion 1. destruct H as [[Heq HΦ] H]. cbn in H.
+    destruct H as (ρ & Hpreds & Hindpreds & Heval); cbn in *. destruct x; cbn in *.
+    subst indcons; cbn in *. apply IHα.
+    destruct α.
+    + cbn. 
+Admitted.
+
+Lemma ODD_φ_Φ_ω : forall n, ODD n -> @φ_Φ_ω Σ__PA M__PA Φ__PA PA_O (V.cons n V.nil).
+Proof.
+  intros n HO. induction HO using ODD_ind2.
+  - exists 2. unfold φ_Φ_n, φ_Φ, φ_P; cbn. exists PA_prod_O_succ, (conj eq_refl ID_O_succ); cbn.
+    unfold φ_pr; cbn. exists (fun x => x); cbn; intuition.
+    injection H0; intros Heq; subst.
+    exists PA_prod_E_zero, (conj eq_refl ID_E_zero); cbn.
+    exists (fun x => x); cbn; intuition. apply inj_pair2 in H0; subst; reflexivity.
+  - destruct IHHO as [a Ha]; exists (S (S a)).
+    cbn; unfold φ_Φ, φ_P at 1.
+    exists PA_prod_O_succ; cbn. exists (conj eq_refl ID_O_succ).
+    unfold φ_pr; cbn.
+    exists (fun x => S n); cbn; intuition.
+    injection H0; intros Heq; subst.
+    apply inj_pair2 in H0; subst; cbn.
+    exists PA_prod_E_succ, (conj eq_refl ID_E_succ); cbn.
+    unfold φ_pr; cbn; exists (fun x => n); cbn; intuition.
+    injection H0; intros Heq; subst.
+    apply inj_pair2 in H0; subst; assumption.
+Qed.   
+    
 Lemma standard_model__PA : @standard_model Σ__PA Φ__PA M__PA.
+Proof.
+  unfold standard_model. intros []; cbn; intros ts; split; intros H.
+  - rewrite V.eta. remember (V.tl ts) as tail. cbn in *. pose proof (V.nil_spec tail).
+    subst. rewrite H0. apply NAT_φ_Φ_ω.
+  - apply NAT_all.
+  - rewrite V.eta. remember (V.tl ts) as tail. cbn in *. pose proof (V.nil_spec tail).
+    subst. rewrite H0. apply EVEN_φ_Φ_ω. assumption.
+  - apply φ_Φ_ω_EVEN. rewrite (V.eta ts) in H. pose proof (V.nil_spec (V.tl ts)).
+    rewrite H0 in H. assumption.
+  - rewrite V.eta. remember (V.tl ts) as tail. cbn in *. pose proof (V.nil_spec tail).
+    subst. rewrite H0. apply ODD_φ_Φ_ω. assumption.
+  - admit.
 Admitted.
